core/SyntaxCertification.v
@@ -24,7 +24,7 @@ Instance CoqTLSyntax :
       Rule_getOutputPatternElements := r_outputPattern;
 
       TraceLink_getSourcePattern := TraceLink_getSourcePattern;
-      TraceLink_getIterator := TraceLink_getIterator;
+      TraceLink_getIteration := TraceLink_getIteration;
       TraceLink_getName := TraceLink_getName;
       TraceLink_getTargetElement := target ;    
       
